Extraction now better than ever!

Extraction/main.ml
@@ -1,4 +1,5 @@
 open Extracted;;
+open Printf;;
 open Coq_i8051_Component;;
 open Core.Std;;
 open List;;
@@ -13,36 +14,6 @@ let explode s =
 	if i < 0 then l else exp (i - 1) (s.[i] :: l) in
   exp (String.length s - 1) [];;
 
-(* let program = *)
-(*   let l = (read Sys.argv.(1) ) in *)
-(*   let p = List.map l  explode in *)
-(*   p;; *)
-
-(* let rec print_char_list p = *)
-(*   match p with *)
-(*   | x :: r -> *)
-(* 	 print_char x; *)
-(* 	 print_char_list r; *)
-(*   | [] -> print_char '\n';; *)
-(* let rec print_load_list p = *)
-(*   match p with *)
-(*   | (x,y) :: r -> *)
-(* 	 print_string "("; *)
-(* 	 print_int (Big.to_int x); *)
-(* 	 print_string ","; *)
-(* 	 print_int (Big.to_int y); *)
-(* 	 print_string ")\n"; *)
-(* 	 print_load_list r; *)
-(*   | [] -> print_char '\n';; *)
-
-(* let load_inst = List.map program (fun x -> ihx_to_byte_assoc_line x None (Some []));; *)
-
-
-(* List.iter program  print_char_list ;; *)
-
-(* List.map load_inst (fun f -> match f with *)
-(* | Some insts -> print_load_list insts; *)
-(* | None -> ()) ;; *)
 
 let to_Big x =
   let rec f a b =
@@ -50,25 +21,41 @@ let to_Big x =
   | 0 -> b
   | a' -> f (a-1) (Big.succ b) in
   f x Big.zero;;
-			
-
+		
+let  pl (x : (int8 * int8 list) list) =
+  print_string "[";
+  let rec outer = function
+	| (a, b)::x' ->
+	   Printf.printf "(%i,[" (Big.to_int a);
+	   let rec inner = function
+		 | n::n' ->
+			Printf.printf "%i," (Big.to_int n);
+			inner n'
+		 | [] -> print_string "]),\n"
+	   in
+	   inner b;
+	   outer x'
+	| [] -> print_string "]\n" in
+  outer x
+  
   let () =
 	let program =  List.map (explode (read Sys.argv.(1) )) conv_char in
 	match hd program with
 	| Some i ->
-	   print_int (int_of_string Sys.argv.(2));
+	   let fuel = (int_of_string Sys.argv.(2)) in
 	   print_string "\nGot a program!\n";
 	   print_int (Big.to_int i);
 	   print_string " <- Byte from program\n";
-	   let v = (computeitBinString (to_Big (int_of_string Sys.argv.(2))) program) in
-	   print_string "done\n";
-	   match v with
-	   | Some i ->
-		  print_string "Got: ";
-		  print_int  (Big.to_int i);
-		  print_string "\n";
-		  ()
-	   | None ->
-		  print_string"No Result\n";
-		  ()
+	   let d = BB.demo3  program (to_Big 6) in
+	   pl (IORUN.run d (to_Big fuel))
+	   (* print_string "done\n"; *)
+	   (* match v with *)
+	   (* | Some i -> *)
+	   (* 	  print_string "Got: "; *)
+	   (* 	  print_int  (Big.to_int i); *)
+	   (* 	  print_string "\n"; *)
+	   (* 	  () *)
+	   (* | None -> *)
+	   (* 	  print_string"No Result\n"; *)
+	   (* 	  () *)
   | None -> print_string "No Program?\n";;
