ctest/test.asm
@@ -1,0 +1,6 @@
+	ljmp main						;
+	
+	.org 100h
+	main:
+	setb p3.1
+	ljmp main
