Connect/Breadboard.v
@@ -1,3 +1,4 @@
+
 Require Import String.
 Require Import Ascii.
 Require Import List.
@@ -7,65 +8,111 @@ Import ListNotations.
 Require Import Arith.
 Open Scope list_scope.
 Open Scope string_scope.
+Add LoadPath "../Model".
 
-(* Notation "$ x" := (fun f => f x) (at level 0, right associativity, only parsing). *)
-(* Notation "f $ x .. y" := (.. (f x) .. y) (at level 0, right associativity, only parsing). *)
 Require Import Common.
 Require Import IOModule.
 Require Import Run.
 Import IORUN.
 Import Wires.
+Require Import c8051.
+Import i8051_Component.
+
+Module BB.
+  (* Module Integrator_Spec. *)
+  (*   Definition io (x:list IO.t):IO.t := suml x. *)
+  (* End Integrator_Spec. *)
+  (* Module Incrementor_Spec. *)
+  (*   Definition io (x:list IO.t):IO.t := len x. *)
+  (* End Incrementor_Spec. *)
 
 
-(* Module Integrator_Spec. *)
-(*   Definition io (x:list IO.t):IO.t := suml x. *)
-(* End Integrator_Spec. *)
-(* Module Incrementor_Spec. *)
-(*   Definition io (x:list IO.t):IO.t := len x. *)
-(* End Incrementor_Spec. *)
+  Fixpoint alt x start:=
+    match x with
+      | O => start
+      | S n => alt n (if beq_nat start 0 then 1 else 0)
+    end.
+  (* Module Alternator_Spec. *)
+  (*   Require Import Arith.Even. *)
+  (*   Definition io (x:list IO.t):IO.t := alt (length x) 1. *)
+  (* End Alternator_Spec. *)
+
+  (* Module Integrator := Component(IO)(Integrator_Spec). *)
+  (* Module Incrementor := Component(IO)(Incrementor_Spec). *)
+  (* Module Alternator := Component(IO)(Alternator_Spec). *)
 
 
-Fixpoint alt x start:=
-  match x with
-    | O => start
-    | S n => alt n (if beq_nat start 0 then 1 else 0)
-  end.
-(* Module Alternator_Spec. *)
-(*   Require Import Arith.Even. *)
-(*   Definition io (x:list IO.t):IO.t := alt (length x) 1. *)
-(* End Alternator_Spec. *)
+  Definition integrator  : IO.func := IO.fn_args 1 (fun x =>suml (hd [] x)).
+  Definition incrementor :IO.func := IO.fn_args 1
+                                                (fun x =>len (hd [] x)).
+  Definition alternator : IO.func :=IO.fn_args 1
+                                               (fun x =>
+                                                  alt (length (hd [] x)) 1).
+  Definition zero_rail   : IO.func := IO.fn_args 0 (fun _ =>0).
 
-(* Module Integrator := Component(IO)(Integrator_Spec). *)
-(* Module Incrementor := Component(IO)(Incrementor_Spec). *)
-(* Module Alternator := Component(IO)(Alternator_Spec). *)
+  Definition delay_n n default : IO.func := IO.fn_args 1
+                                                       (fun x => nth n (hd [] x) default).
 
 
-Definition integrator  : IO.func := IO.fn_args 1 (fun x =>suml (hd [] x)).
-Definition incrementor :IO.func := IO.fn_args 1
-                                              (fun x =>len (hd [] x)).
-Definition alternator : IO.func :=IO.fn_args 1
-                                             (fun x =>
-                                                alt (length (hd [] x)) 1).
-Definition zero_rail   : IO.func := IO.fn_args 0 (fun _ =>0).
+  Open Scope wiring_scope.
 
-Definition delay_n n default : IO.func := IO.fn_args 1
-                                                     (fun x => nth n (hd [] x) default).
+  Definition demo1 := base */  zero_rail ~> 0
+                           //  [5] ~> integrator~> 6
+                           // [2] ~> integrator~> 3
+                           */ incrementor ~> 2
+                           */ IO.fn_args 0 (fun _=> 10) ~> 5
+                           */ alternator ~> 8
+                           # 3 "Integrated incrementor"
+                           # 3 "Integrated incrementor".
 
-
-Open Scope wiring_scope.
-
-Definition demo1 := base */  zero_rail ~> 0
-                         //  [5] ~> integrator~> 6
-                         // [2] ~> integrator~> 3
-                         */ incrementor ~> 2
-                         */ IO.fn_args 0 (fun _=> 10) ~> 5
-                         */ alternator ~> 8
-                         # 3 "Integrated incrementor"
-                         # 3 "Integrated incrementor".
-
-Compute (docstring demo1).
-Definition demo2 := base */integrator ~> 9
-                         // [6] ~> delay_n 5 0 ~> 10.
+  Compute (docstring demo1).
+  Definition demo2 := base */integrator ~> 9
+                           // [6] ~> delay_n 5 0 ~> 10.
 
 
 
+
+  Definition demo3 bin threshold  :=
+    base // (seq 0 32) ~> i8051_Component bin threshold dac ~> 32
+         ~&~
+         base */ zero_rail ~> 0
+         */ zero_rail ~> 1
+         */ zero_rail ~> 2
+         */ zero_rail ~> 3
+         */ zero_rail ~> 4
+         */ zero_rail ~> 5
+         */ zero_rail ~> 6
+         */ zero_rail ~> 7
+         */ zero_rail ~> 8
+         */ zero_rail ~> 9
+         */ zero_rail ~> 10
+         */ zero_rail ~> 11
+         */ zero_rail ~> 12
+         */ zero_rail ~> 13
+         */ zero_rail ~> 14
+         */ zero_rail ~> 15
+         */ zero_rail ~> 16
+         */ zero_rail ~> 17
+         */ zero_rail ~> 18
+         */ zero_rail ~> 19
+         */ zero_rail ~> 20
+         */ zero_rail ~> 21
+         */ zero_rail ~> 22
+         */ zero_rail ~> 23
+         */ zero_rail ~> 24
+         */ zero_rail ~> 25
+         */ zero_rail ~> 26
+         */ zero_rail ~> 27
+         */ zero_rail ~> 28
+         */ zero_rail ~> 29
+         */ zero_rail ~> 30
+         */ zero_rail ~> 31 .
+
+  Definition run := run.
+
+  Lemma valid_demo3: valid_wiring (demo3 [0] 6).
+    admit. (* THis works just slowly *)
+    (* autowire. *)
+
+  Qed.
+End BB.
