Connect/c8051.v
@@ -13,35 +13,38 @@ Require Import ZArith.
 Require Import i8051Semantics.
 Require Import i8051Syntax.
 Import i8051_MACHINE.
-Definition default := {| executing := NOP;
-                         pc := Word.repr 0;
-                         cycle := 0;
-                         output := {| P0:=Word.repr 0;P1:=Word.repr 0;P2:=Word.repr 0;P3:=Word.repr 0 |}
-                      |}.
+(* Definition default := {| executing := NOP; *)
+(*                          pc := Word.repr 0; *)
+(*                          cycle := 0; *)
+(*                          output := {| P0:=Word.repr 0;P1:=Word.repr 0;P2:=Word.repr 0;P3:=Word.repr 0 |} *)
+(*                       |}. *)
 Definition m_init   :=  {|
                         pc_reg := Word.repr  0;
-                        trace := [];
-                        external := (fun tr => let t := hd  default tr in 
-                                              {| executing := executing t;
-                                                 pc := pc t;
-                                                 cycle := cycle t;
-                                                 output := {| P0:=Word.repr 0;P1:=Word.repr 0;P2:=Word.repr 0;P3:=Word.repr 0 |}
+                        (* trace := []; *)
+                        external :=
+                          {| P0:=Word.repr 0;P1:=Word.repr 0;P2:=Word.repr 0;P3:=Word.repr 0 |}|}.
 
-                                              |})
-                      |}.
+(*     (fun tr => let t := hd  default tr in  *)
+(*                         {| executing := executing t; *)
+(*                            pc := pc t; *)
+(*                            cycle := cycle t; *)
+(*                            output := {| P0:=Word.repr 0;P1:=Word.repr 0;P2:=Word.repr 0;P3:=Word.repr 0 |} *)
+
+(*                         |}) *)
+(* |}. *)
 Import i8051_RTL.
 Definition oracle := {|
-    oracle_bits := Word.repr ; 
-    oracle_offset := 0
-  |}.
-  Definition r := {|
-    rtl_oracle := oracle ; 
-    rtl_env := empty_env ; 
-    rtl_mach_state := m_init; 
-    rtl_memory := AddrMap.init (Word.repr 0);
-    rtl_code := CodeMap.init (Word.repr 0)
-  |}. 
-  
+                      oracle_bits := Word.repr ; 
+                      oracle_offset := 0
+                    |}.
+Definition r := {|
+                 rtl_oracle := oracle ; 
+                 rtl_env := empty_env ; 
+                 rtl_mach_state := m_init; 
+                 rtl_memory := AddrMap.init (Word.repr 0);
+                 rtl_code := CodeMap.init (Word.repr 0)
+               |}. 
+
 Module i8051_Component.
   (* Variable threshold : nat. *)
   Definition threshold := 1.
@@ -62,26 +65,88 @@ Module i8051_Component.
 
   
 
-  Definition computeit cycle init := dump_state cycle {|
-    rtl_oracle :=  {|
-    oracle_bits := Word.repr ; 
-    oracle_offset := 0
-  |}; 
-    rtl_env := empty_env ; 
-    rtl_mach_state := m_init; 
-    rtl_memory := AddrMap.init (Word.repr 0);
-    rtl_code := CodeMap.init (Word.repr 0)
-  |} init.
-  Definition computeitIHXString cycle init := 
-    let loads := flat_map (fun x =>
-                             match ihx_to_byte_assoc_line (asciis x) None (Some nil) with
-                               | Some v => v
-                               | None => nil
-                             end) init in
-    computeit cycle  (load_code_bytes loads).
-  Definition computeitBinString cycle init := 
-    computeit cycle  (load_code_bytes_bin init 0).
+  Definition run_8051 init ps := dump_state  {|
+                                                    rtl_oracle :=  {|
+                                                                   oracle_bits := Word.repr ; 
+                                                                   oracle_offset := 0
+                                                                 |}; 
+                                                    rtl_env := empty_env ; 
+                                                    rtl_mach_state := m_init; 
+                                                    rtl_memory := AddrMap.init (Word.repr 0);
+                                                    rtl_code := CodeMap.init (Word.repr 0)
+                                                  |} ps init.
+  (* Definition computeitIHXString cycle init :=  *)
+  (*   let loads := flat_map (fun x => *)
+  (*                            match ihx_to_byte_assoc_line (asciis x) None (Some nil) with *)
+  (*                              | Some v => v *)
+  (*                              | None => nil *)
+  (*                            end) init in *)
+  (*  run8051 cycle  (load_code_bytes loads). *)
+  Definition run_8051_bin_string bin ps := 
+    run_8051 (load_code_bytes_bin bin 0) ps.
+  SearchAbout nat.
+  SearchAbout Word.int.
+  Definition condense (b7 b6 b5 b4 b3 b2 b1 b0: bool) :=
+    let i7 : int8 := Word.bool_to_int b7 in
+    let i6 : int8 := Word.bool_to_int b6 in
+    let i5 : int8 := Word.bool_to_int b5 in
+    let i4 : int8 := Word.bool_to_int b4 in
+    let i3 : int8 := Word.bool_to_int b3 in
+    let i2 : int8 := Word.bool_to_int b2 in
+    let i1 : int8 := Word.bool_to_int b1 in
+    let i0 : int8 := Word.bool_to_int b0 in
+    fold_left (fun s f => Word.or (Word.shl s (Word.repr 1))  f) [i7;i6;i5;i4;i3;i2;i1;i0] Word.zero.
+
+  Fixpoint condense' l7 l6 l5 l4 l3 l2 l1 l0 :=
+    match l7, l6, l5, l4, l3, l2, l1, l0  with
+        | a::a',b::b',c::c',d::d',e::e',f::f',g::g',h::h' => (condense a b c d e f g h) :: (condense' a' b' c' d' e' f' g' h')
+        | _,_,_,_,_,_,_,_ => []
+    end.
+  
+  Fixpoint to_trace p1 p2 p3 p4 :=
+    match p1, p2, p3, p4 with
+      | a::a', b::b', c::c', d::d' => {| P0 := a; P1 := b; P2:=c;P3:=d |} :: to_trace a' b' c' d'
+      | _,_,_,_ => []
+    end.
+
+  Definition traces (tr:trace) thresh :=
+    let digitized := map (map (fun x => NPeano.ltb x thresh)) tr in
+    
+    match digitized with
+        |(p00::p01::p02::p03::p04::p05::p06::p07::
+           p10::p11::p12::p13::p14::p15::p16::p17::
+           p20::p21::p22::p23::p24::p25::p26::p27::
+           p30::p31::p32::p33::p34::p35::p36::p37::nil) =>
+         
+        to_trace (condense' p07 p06 p05 p04 p03 p02 p01 p00)
+         (condense' p17 p16 p15 p14 p13 p12 p11 p10)
+         (condense' p27 p26 p25 p24 p23 p22 p21 p20)
+         (condense' p37 p36 p35 p34 p33 p32 p31 p30)
+        |_ => []
+    end.
+        
+
+    
+
+    
+  Definition i8051_Component bin threshold conv:=
+    fn_args (8*4) (fun t =>
+                     let ps := traces t threshold in
+                     conv (run_8051_bin_string bin ps)).
+  
   Require Import Ascii.
   Definition conv_char (c:ascii) : int8 := Word.repr (Z_of_nat (nat_of_ascii c)).
+Check i8051_Component.
 End i8051_Component.
-
+Compute (seq 0 32).
+Import i8051_Component.
+SearchAbout Word.int.
+Check Z.to_N.
+Search nat.
+Definition dac x := match x with
+					  | Some v =>
+						let z := P3 v in
+						N.to_nat(    Z.to_N (Word.unsigned (Word.and z (Word.not (Word.repr 1)))))
+                      | None => 0
+                    end.
+Check dac.
