Model/RTL.v
@@ -43,9 +43,6 @@ Module Type MACHINE_SIG.
   (** And operations for reading/writing locations *)
   Variable get_location : forall s, location s -> mach_state -> Word.int s.
   Variable set_location : forall s, location s -> Word.int s -> mach_state -> mach_state.
-  Variable trace_type :Type.
-  Variable get_trace: mach_state -> list trace_type.
-  Variable add_trace: trace_type -> mach_state -> mach_state.
 End MACHINE_SIG.
 
 (** Generic register-transfer language *)    
@@ -109,7 +106,6 @@ Module RTL(M : MACHINE_SIG).
   | set_byte_rtl: forall (rs:pseudo_reg size8)(addr:pseudo_reg size_addr), rtl_instr
   | get_byte_rtl: forall (addr:pseudo_reg size_addr)(rd:pseudo_reg size8), rtl_instr
   | choose_rtl : forall s (rd:pseudo_reg s), rtl_instr
-  | add_trace_rtl : forall (t:trace_type), rtl_instr
   | error_rtl : rtl_instr
   | safe_fail_rtl : rtl_instr.
 
@@ -186,12 +182,6 @@ Module RTL(M : MACHINE_SIG).
                            rtl_code := rtl_code rs ; 
                            rtl_memory := rtl_memory rs |}).
 
-  Definition add_tr (t : trace_type) : RTL unit := 
-    fun rs => (Okay_ans tt, {| rtl_oracle := rtl_oracle rs ; 
-                           rtl_env := rtl_env rs ; 
-                           rtl_mach_state := add_trace t (rtl_mach_state rs) ; 
-                           rtl_code := rtl_code rs ; 
-                           rtl_memory := rtl_memory rs |}).
   Definition set_byte (addr:int size_addr) (v:int size8) : RTL unit := 
     fun rs => (Okay_ans tt, {| rtl_oracle := rtl_oracle rs ; 
                            rtl_env := rtl_env rs ; 
@@ -274,7 +264,6 @@ Module RTL(M : MACHINE_SIG).
       | set_byte_rtl rs addr => v <- get_ps rs ; a <- get_ps addr ; set_byte a v
       | get_byte_rtl addr rd => a <- get_ps addr ; v <- get_byte a ; set_ps rd v
       | choose_rtl s rd => v <- choose_bits s ; set_ps rd v
-      | add_trace_rtl a => add_tr a
       | error_rtl => Fail unit
       | safe_fail_rtl => SafeFail unit
     end.
